First drafts of implicit typing

verification/Context.v
@@ -1,15 +1,18 @@
 (*
-    Here the typing rules of the system are defined. We also define some
-    main facts, but don't prove them here. For proofs see `TypingAndReduction.v`
+    The library with facts about lifting, lowering and 
+    substitution in contexts. True for all versions
+    of our system
 *)
-Require Import Program.Equality.
-
-Require List.
 Require Import Term.
+Require Import Omega.
 Require Import String.
 Require Import ListLemmas.
-Require Import TermReduction.
 
+(* TODO: shorten the file by using some general facts *)
+
+(*
+    Following the Pierce's impl, we save the var's name too.
+*)
 Definition context : Set := list (option (string * term)).
 
 Definition lift_ctx_elem (c d : nat) (x : option (string * term)) : option (string * term) :=
@@ -77,244 +80,6 @@ Notation "G [ x ] := ?!" := (has_no_type G x) (at level 70, no associativity).
 
 (* A notation for pushing variables. Note that it conflicts with list *)
 Notation "{ s == x } :: G" := (push_var G s x) (at level 84, no associativity).
-
-Reserved Notation "G |- x := y" (at level 85, no associativity).
-
-(* Typing rules *)
-Inductive typing : context -> term -> term -> Prop :=
-(* Core typing *)
-| TNat :
-    forall (ctx : context),
-    WF ctx ->
-    ctx |- Nat := SmallKind
-| TNatO : 
-    forall (ctx : context),
-    WF ctx ->
-    ctx |- NatO := Nat
-| TNatSucc : 
-    forall (ctx : context),
-    WF ctx ->
-    ctx |- NatSucc := Forall "_"%string Nat Nat
-| TNatRec : 
-    forall (ctx : context),
-    forall choice zero step num : term,
-    ctx |- choice := Nat ===> SmallKind -> 
-    ctx |- zero := App choice NatO ->
-    ctx |- step := Forall "n"%string Nat (App (lift choice 0 1) (Var 0) ===> App (lift choice 0 2) (App NatSucc (Var 1))) ->
-    ctx |- num := Nat ->
-    ctx |- NatRec choice zero step num := App choice num
-| TApp : 
-    forall (ctx : context),
-    forall (str : string) (domain range : term) (l r : term),
-    ctx |- l := Forall str domain range ->
-    ctx |- r := domain ->
-    ctx |- App l r := top_subst range r
-| TAbsSmall : 
-    forall (ctx : context),
-    forall (str : string) (range : term) (arg_type body : term),
-    ctx |- arg_type := SmallKind ->
-    push_var ctx str arg_type |- body := range ->
-    ctx |- Abs str arg_type body := Forall str arg_type range
-| TAbsType : 
-    forall (ctx : context),
-    forall (str : string) (range : term) (arg_type body : term) (i : nat),
-    ctx |- arg_type := TypeKind i ->
-    { str == arg_type } :: ctx |- body := range ->
-    ctx |- Abs str arg_type body := Forall str arg_type range
-| TAbsProp : 
-    forall (ctx : context),
-    forall (str : string) (range : term) (arg_type body : term),
-    ctx |- arg_type := PropKind ->
-    { str == arg_type } :: ctx |- body := range ->
-    ctx |- Abs str arg_type body := Forall str arg_type range
-| TVar : 
-    forall (ctx : context),
-    forall (n : nat) (t : term), 
-    WF ctx -> 
-    ctx[n] := t -> 
-    ctx |- Var n := t
-| TSmallKind : 
-    forall (ctx : context),
-    WF ctx -> 
-    ctx |- SmallKind := TypeKind 0
-| TPropKind :
-    forall (ctx : context),
-    WF ctx -> 
-    ctx |- PropKind := TypeKind 0
-| TTypeKind : 
-    forall (ctx : context),
-    WF ctx -> 
-    forall n : nat, ctx |- TypeKind n := TypeKind (S n)
-| TForallType : 
-    forall (ctx : context),
-    forall (str : string) (domain range : term) (universe : nat),
-    ctx |- domain := TypeKind universe ->
-    { str == domain } :: ctx |- range := TypeKind universe ->
-    ctx |- Forall str domain range := TypeKind universe
-| TForallPropSmall : 
-    forall (ctx : context),
-    forall (str : string) (domain range : term),
-    ctx |- domain := SmallKind ->
-    { str == domain } :: ctx |- range := PropKind ->
-    ctx |- Forall str domain range := PropKind
-| TForallPropProp : 
-    forall (ctx : context),
-    forall (str : string) (domain range : term),
-    ctx |- domain := PropKind ->
-    { str == domain } :: ctx |- range := PropKind ->
-    ctx |- Forall str domain range := PropKind
-| TForallPropType : 
-    forall (ctx : context),
-    forall (str : string) (domain range : term),
-    forall (i : nat), ctx |- domain := TypeKind i ->
-    { str == domain } :: ctx |- range := PropKind ->
-    ctx |- Forall str domain range := PropKind
-| TForallSmallSmall : 
-    forall (ctx : context),
-    forall (str : string) (domain range : term),
-    ctx |- domain := SmallKind ->
-    { str == domain } :: ctx |- range := SmallKind ->
-    ctx |- Forall str domain range := SmallKind
-| TForallSmallProp : 
-    forall (ctx : context),
-    forall (str : string) (domain range : term),
-    ctx |- domain := PropKind ->
-    { str == domain } :: ctx |- range := SmallKind ->
-    ctx |- Forall str domain range := SmallKind
-(* Universe transition rules *)
-| JumpToTypeUniverseSmall :
-    forall (ctx : context),
-    forall (t : term),
-    ctx |- t := SmallKind ->
-    ctx |- t := TypeKind 0
-| JumpToTypeUniverseProp :
-    forall (ctx : context),
-    forall (t : term),
-    ctx |- t := PropKind ->
-    ctx |- t := TypeKind 0
-| RaiseUniverse : 
-    forall (ctx : context),
-    forall (t : term) (universe : nat),
-    ctx |- t := TypeKind universe ->
-    ctx |- t := TypeKind (S universe)
-(* Conversion axioms *)
-| ConversionSmallL : 
-    forall (ctx : context),
-    forall (t : term) (type type' : term),
-    ctx |- t := type ->
-    ctx |- type := SmallKind ->
-    type ->b type' ->
-    ctx |- type' := SmallKind ->
-    ctx |- t := type'
-| ConversionPropL : 
-    forall (ctx : context),
-    forall (t : term) (type type' : term),
-    ctx |- t := type ->
-    ctx |- type := PropKind ->
-    type ->b type' ->
-    ctx |- type' := PropKind ->
-    ctx |- t := type'
-| ConversionTypeL : 
-    forall (ctx : context),
-    forall (t : term) (type type' : term) (i : nat),
-    ctx |- t := type ->
-    ctx |- type := TypeKind i ->
-    type ->b type' ->
-    ctx |- type' := TypeKind i ->
-    ctx |- t := type'
-| ConversionSmallR : 
-    forall (ctx : context),
-    forall (t : term) (type type' : term),
-    ctx |- t := type ->
-    ctx |- type := SmallKind ->
-    type' ->b type ->
-    ctx |- type' := SmallKind ->
-    ctx |- t := type'
-| ConversionPropR : 
-    forall (ctx : context),
-    forall (t : term) (type type' : term),
-    ctx |- t := type ->
-    ctx |- type := PropKind ->
-    type' ->b type ->
-    ctx |- type' := PropKind ->
-    ctx |- t := type'
-| ConversionTypeR : 
-    forall (ctx : context),
-    forall (t : term) (type type' : term) (i : nat),
-    ctx |- t := type ->
-    ctx |- type := TypeKind i ->
-    type' ->b type ->
-    ctx |- type' := TypeKind i ->
-    ctx |- t := type'
-| ConversionSmallRename : 
-    forall (ctx : context),
-    forall (t : term) (type type' : term),
-    ctx |- t := type ->
-    ctx |- type := SmallKind ->
-    type =a type' ->
-    ctx |- type' := SmallKind ->
-    ctx |- t := type'
-| ConversionPropRename : 
-    forall (ctx : context),
-    forall (t : term) (type type' : term),
-    ctx |- t := type ->
-    ctx |- type := PropKind ->
-    type =a type' ->
-    ctx |- type' := PropKind ->
-    ctx |- t := type'
-| ConversionTypeRename : 
-    forall (ctx : context),
-    forall (t : term) (type type' : term) (i : nat),
-    ctx |- t := type ->
-    ctx |- type := TypeKind i ->
-    type =a type' ->
-    ctx |- type' := TypeKind i ->
-    ctx |- t := type'
-(* Well formed context axioms *)
-with WF : context -> Prop :=
-| WF_empty : WF nil
-| WF_assum_small : 
-    forall (ctx : context) (str : string) (t : term),
-    WF ctx ->
-    ctx |- t := SmallKind ->
-    WF (push_var ctx str t)
-| WF_assum_prop :
-    forall (ctx : context) (str : string) (t : term),
-    WF ctx ->
-    ctx |- t := PropKind ->
-    WF (push_var ctx str t)
-| WF_assum_type :
-    forall (ctx : context) (str : string) (t : term) (i : nat),
-    WF ctx ->
-    ctx |- t := TypeKind i ->
-    WF (push_var ctx str t)
-| WF_dummy_assum :
-    forall (ctx : context),
-    WF ctx ->
-    WF (push_dummy ctx)
-
-where "G |- x := y" := (typing G x y)
-.
-
-(* Induction scheme when the simple induction won't do the trick *)
-Scheme typing_ind_mut := Induction for 
-typing Sort Prop
-with wf_ind_mut := Induction for 
-WF Sort Prop.
-
-Ltac depind_typing WF_inv H := (do_depind ltac:(fun x => induction x using (fun x => typing_ind_mut x WF_inv)) H).
-
-Definition typable (ctx : context) (t : term) := exists type : term, ctx |- t := type.
-Notation "G |- x := ?" := (typable G x) (at level 85, no associativity).
-
-Theorem typable_wf : forall (ctx : context) (t type : term),
-    ctx |- t := type ->
-    WF ctx
-.
-Proof.
-    intros.
-    induction H; try easy.
-Qed.
 
 Lemma lift_context_split : forall (l r : context) (c d : nat),
     lift_context (l ++ r)%list c d = (lift_context l c d ++ lift_context r c d)%list
@@ -527,86 +292,6 @@ Proof.
     apply (lift_lemma_None _ c d) in H0.
     intro H1.
     exfalso; exact (has_type_contradict _ _ _ H1 H0).
-Qed.
-
-Lemma wf_ctx_slot_lt_var : forall (ctx : context),
-    WF ctx ->
-    (
-        forall (slot : nat) (t : term),
-        ctx[slot] := t ->
-        (forall v, var_occurs t v -> slot < v)
-    )
-.
-Proof.
-    intros ctx H.
-    induction H; intros.
-
-    unfold has_type in H.
-    destruct slot; easy.
-
-    destruct slot.
-    unfold has_type in H1; simpl in H1.
-    subst t0.
-    destruct v.
-    exfalso; generalize H2; apply (lifting_destroys _ _ _ _ (Le.le_0_n _) (PeanoNat.Nat.lt_0_succ _)).
-    apply PeanoNat.Nat.lt_0_succ.
-    change (({str == t} :: ctx)[S slot] := t0) with ((lift_context ctx 0 1)[slot] := t0) in H1.
-    destruct (ctx_var_lifted_repr _ _ _ _ _ H1).
-    subst t0.
-    destruct v.
-    exfalso; generalize H2; apply (lifting_destroys _ _ _ _ (Le.le_0_n _) (PeanoNat.Nat.lt_0_succ _)).
-    apply Lt.lt_n_S.
-    rewrite <- (PeanoNat.Nat.add_1_r v) in H2.
-    apply (lifting_respects_occurance_r _ _ _ _ (Le.le_0_n _)) in H2.
-    apply lift_lemma_Some in H1.
-    exact (IHWF _ _ H1 _ H2).
-
-    destruct slot.
-    unfold has_type in H1; simpl in H1.
-    subst t0.
-    destruct v.
-    exfalso; generalize H2; apply (lifting_destroys _ _ _ _ (Le.le_0_n _) (PeanoNat.Nat.lt_0_succ _)).
-    apply PeanoNat.Nat.lt_0_succ.
-    change (({str == t} :: ctx)[S slot] := t0) with ((lift_context ctx 0 1)[slot] := t0) in H1.
-    destruct (ctx_var_lifted_repr _ _ _ _ _ H1).
-    subst t0.
-    destruct v.
-    exfalso; generalize H2; apply (lifting_destroys _ _ _ _ (Le.le_0_n _) (PeanoNat.Nat.lt_0_succ _)).
-    apply Lt.lt_n_S.
-    rewrite <- (PeanoNat.Nat.add_1_r v) in H2.
-    apply (lifting_respects_occurance_r _ _ _ _ (Le.le_0_n _)) in H2.
-    apply lift_lemma_Some in H1.
-    exact (IHWF _ _ H1 _ H2).
-
-    destruct slot.
-    unfold has_type in H1; simpl in H1.
-    subst t0.
-    destruct v.
-    exfalso; generalize H2; apply (lifting_destroys _ _ _ _ (Le.le_0_n _) (PeanoNat.Nat.lt_0_succ _)).
-    apply PeanoNat.Nat.lt_0_succ.
-    change (({str == t} :: ctx)[S slot] := t0) with ((lift_context ctx 0 1)[slot] := t0) in H1.
-    destruct (ctx_var_lifted_repr _ _ _ _ _ H1).
-    subst t0.
-    destruct v.
-    exfalso; generalize H2; apply (lifting_destroys _ _ _ _ (Le.le_0_n _) (PeanoNat.Nat.lt_0_succ _)).
-    apply Lt.lt_n_S.
-    rewrite <- (PeanoNat.Nat.add_1_r v) in H2.
-    apply (lifting_respects_occurance_r _ _ _ _ (Le.le_0_n _)) in H2.
-    apply lift_lemma_Some in H1.
-    exact (IHWF _ _ H1 _ H2).
-
-    destruct slot.
-    unfold has_type in H1; simpl in H1; easy.
-    change ((push_dummy ctx)[S slot] := t) with ((lift_context ctx 0 1)[slot] := t) in H0.
-    destruct (ctx_var_lifted_repr _ _ _ _ _ H0).
-    subst t.
-    destruct v.
-    exfalso; generalize H1; apply (lifting_destroys _ _ _ _ (Le.le_0_n _) (PeanoNat.Nat.lt_0_succ _)).
-    apply Lt.lt_n_S.
-    rewrite <- (PeanoNat.Nat.add_1_r v) in H1.
-    apply (lifting_respects_occurance_r _ _ _ _ (Le.le_0_n _)) in H1.
-    apply lift_lemma_Some in H0.
-    exact (IHWF _ _ H0 _ H1).
 Qed.
 
 Lemma lift_lower_context_destruct : forall (ctx : context) (c d : nat),
@@ -854,142 +539,6 @@ Proof.
     now apply IHctx.
 Qed.
 
-Lemma var_used_ineq : forall (l r : context) (v : nat),
-    WF (l ++ r)%list ->
-    var_used r v -> List.length l <= v
-.
-Proof.
-    intros l r v H.
-    generalize v; clear v; dependent induction H; intros.
-
-    symmetry in x; apply List.app_eq_nil in x.
-    destruct x; subst r; simpl in H0; easy.
-
-    destruct l.
-    simpl; apply le_0_n.
-    simpl in x; simpl.
-    unfold push_var in x; simpl in x.
-    injection x; intros.
-    destruct v.
-    assert (var_used (l ++ r)%list 0).
-    apply var_used_cases; tauto.
-    exfalso; generalize H4.
-    rewrite <- H2.
-    unfold lift1_context.
-    apply (lifting_context_destroys _ _ _ _ (le_0_n _) (PeanoNat.Nat.lt_0_succ _)).
-    apply Le.le_n_S.
-    rewrite <- (lower_context_length l 0 1).
-    apply (IHWF _ (lower_context r 0 1)).
-    rewrite <- lower_context_split.
-    rewrite <- H2.
-    unfold lift1_context; now rewrite lift_lower_context_destruct.
-    elim (lifted_context_repr r 0 1).
-    intros; subst r.
-    rewrite lift_lower_context_destruct.
-    apply (lifting_context_respects_occurance_r _ _ 1 _ (le_0_n _)).
-    now rewrite PeanoNat.Nat.add_1_r.
-    intros.
-    destruct v0.
-    exfalso; cut (var_used (lift1_context ctx) 0).
-    unfold lift1_context.
-    apply (lifting_context_destroys _ _ _ _ (le_0_n _) (PeanoNat.Nat.lt_0_succ _)).
-    rewrite H2; apply var_used_cases; tauto.
-    right; apply Le.le_n_S; apply Le.le_0_n.
-
-    destruct l.
-    simpl; apply le_0_n.
-    simpl in x; simpl.
-    unfold push_var in x; simpl in x.
-    injection x; intros.
-    destruct v.
-    assert (var_used (l ++ r)%list 0).
-    apply var_used_cases; tauto.
-    exfalso; generalize H4.
-    rewrite <- H2.
-    unfold lift1_context.
-    apply (lifting_context_destroys _ _ _ _ (le_0_n _) (PeanoNat.Nat.lt_0_succ _)).
-    apply Le.le_n_S.
-    rewrite <- (lower_context_length l 0 1).
-    apply (IHWF _ (lower_context r 0 1)).
-    rewrite <- lower_context_split.
-    rewrite <- H2.
-    unfold lift1_context; now rewrite lift_lower_context_destruct.
-    elim (lifted_context_repr r 0 1).
-    intros; subst r.
-    rewrite lift_lower_context_destruct.
-    apply (lifting_context_respects_occurance_r _ _ 1 _ (le_0_n _)).
-    now rewrite PeanoNat.Nat.add_1_r.
-    intros.
-    destruct v0.
-    exfalso; cut (var_used (lift1_context ctx) 0).
-    unfold lift1_context.
-    apply (lifting_context_destroys _ _ _ _ (le_0_n _) (PeanoNat.Nat.lt_0_succ _)).
-    rewrite H2; apply var_used_cases; tauto.
-    right; apply Le.le_n_S; apply Le.le_0_n.
-
-    destruct l.
-    simpl; apply le_0_n.
-    simpl in x; simpl.
-    unfold push_var in x; simpl in x.
-    injection x; intros.
-    destruct v.
-    assert (var_used (l ++ r)%list 0).
-    apply var_used_cases; tauto.
-    exfalso; generalize H4.
-    rewrite <- H2.
-    unfold lift1_context.
-    apply (lifting_context_destroys _ _ _ _ (le_0_n _) (PeanoNat.Nat.lt_0_succ _)).
-    apply Le.le_n_S.
-    rewrite <- (lower_context_length l 0 1).
-    apply (IHWF _ (lower_context r 0 1)).
-    rewrite <- lower_context_split.
-    rewrite <- H2.
-    unfold lift1_context; now rewrite lift_lower_context_destruct.
-    elim (lifted_context_repr r 0 1).
-    intros; subst r.
-    rewrite lift_lower_context_destruct.
-    apply (lifting_context_respects_occurance_r _ _ 1 _ (le_0_n _)).
-    now rewrite PeanoNat.Nat.add_1_r.
-    intros.
-    destruct v0.
-    exfalso; cut (var_used (lift1_context ctx) 0).
-    unfold lift1_context.
-    apply (lifting_context_destroys _ _ _ _ (le_0_n _) (PeanoNat.Nat.lt_0_succ _)).
-    rewrite H2; apply var_used_cases; tauto.
-    right; apply Le.le_n_S; apply Le.le_0_n.
-
-    destruct l.
-    simpl; apply le_0_n.
-    simpl in x; simpl.
-    unfold push_var in x; simpl in x.
-    injection x; intros.
-    destruct v.
-    assert (var_used (l ++ r)%list 0).
-    apply var_used_cases; tauto.
-    exfalso; generalize H3.
-    rewrite <- H1.
-    unfold lift1_context.
-    apply (lifting_context_destroys _ _ _ _ (le_0_n _) (PeanoNat.Nat.lt_0_succ _)).
-    apply Le.le_n_S.
-    rewrite <- (lower_context_length l 0 1).
-    apply (IHWF _ (lower_context r 0 1)).
-    rewrite <- lower_context_split.
-    rewrite <- H1.
-    unfold lift1_context; now rewrite lift_lower_context_destruct.
-    elim (lifted_context_repr r 0 1).
-    intros; subst r.
-    rewrite lift_lower_context_destruct.
-    apply (lifting_context_respects_occurance_r _ _ 1 _ (le_0_n _)).
-    now rewrite PeanoNat.Nat.add_1_r.
-    intros.
-    destruct v0.
-    exfalso; cut (var_used (lift1_context ctx) 0).
-    unfold lift1_context.
-    apply (lifting_context_destroys _ _ _ _ (le_0_n _) (PeanoNat.Nat.lt_0_succ _)).
-    rewrite H1; apply var_used_cases; tauto.
-    right; apply Le.le_n_S; apply Le.le_0_n.
-Qed.
-
 Lemma lower_context_c_0 : forall (ctx : context) (c : nat),
     lower_context ctx c 0 = ctx
 .
@@ -1023,40 +572,40 @@ Proof.
 Qed.
 
 Lemma var_used_lift : forall (ctx : context) (c d v : nat),
-    var_used ctx v <-> ((v < c -> var_used (lift_context ctx c d) v) /\ (c <= v -> var_used (lift_context ctx c d) (v + d)))
+    var_used ctx v 
+    <-> 
+    (
+        if Compare_dec.lt_dec v c then var_used (lift_context ctx c d) v
+        else var_used (lift_context ctx c d) (v + d)
+    )
 .
 Proof.
     intro ctx; induction ctx.
-    intros; split; try easy.
-    destruct (PeanoNat.Nat.lt_ge_cases v c); intuition.
+
+    intros.
+    set (H := Compare_dec.lt_dec v c).
+    simpl; tauto.
+
+    intros.
     destruct a.
     destruct p.
     simpl.
-    intros.
-    split.
-    intro H; destruct H.
-    apply (lifting_respects_occurance _ c d v) in H.
-    intuition.
-    apply (IHctx c d v) in H.
-    intuition.
-    intro H; destruct H.
-    destruct (PeanoNat.Nat.lt_ge_cases v c).
-    set (H2 := H H1).
-    destruct H2.
-    apply lifting_respects_occurance_l in H2; tauto.
-    right; apply (IHctx c d v).
-    intuition.
-    exfalso; exact (Lt.lt_not_le _ _ H1 H3).
-    exfalso; exact (Lt.lt_not_le _ _ H1 H3).
-    set (H2 := H0 H1).
-    destruct H2.
-    apply lifting_respects_occurance_r in H2.
+    set (H := lifting_respects_occurance t c d v).
+    set (H0 := IHctx c d v).
+    generalize H H0.
+    set (H1 := Compare_dec.lt_dec v c).
+    assert (
+        (if H1 then (var_occurs (lift t c d) v \/ var_used (lift_context ctx c d) v)
+        else (var_occurs (lift t c d) (v + d) \/ var_used (lift_context ctx c d) (v + d)))
+        =
+        ((if H1 then var_occurs (lift t c d) v
+        else var_occurs (lift t c d) (v + d))
+        \/
+        (if H1 then var_used (lift_context ctx c d) v
+        else var_used (lift_context ctx c d) (v + d)))
+    ) by (now destruct H1).
+    rewrite H2.
     tauto.
-    exact H1.
-    right; apply (IHctx c d v).
-    intuition.
-    exfalso; exact (Lt.lt_not_le _ _ H3 H1).
-    exfalso; exact (Lt.lt_not_le _ _ H3 H1).
     simpl.
     apply IHctx.
 Qed.
@@ -1066,13 +615,9 @@ Lemma var_used_lift_l : forall (ctx : context) (c d v : nat),
     var_used ctx v <-> var_used (lift_context ctx c d) v
 .
 Proof.
-    intros; split.
     intros.
-    exact (proj1 (proj1 (var_used_lift ctx c d v) H0) H).
-    intros.
-    apply (var_used_lift ctx c d v).
-    intuition.
-    exfalso; exact (Lt.lt_not_le _ _ H H1).
+    generalize (var_used_lift ctx c d v).
+    destruct (Compare_dec.lt_dec v c); tauto || omega. 
 Qed.
 
 Lemma var_used_lift_r : forall (ctx : context) (c d v : nat),
@@ -1080,14 +625,9 @@ Lemma var_used_lift_r : forall (ctx : context) (c d v : nat),
     var_used ctx v <-> var_used (lift_context ctx c d) (v + d)
 .
 Proof.
-    intros; split.
     intros.
-    apply (var_used_lift ctx c d v) in H0.
-    exact (proj2 H0 H).
-    intros.
-    apply (var_used_lift ctx c d v).
-    intuition.
-    exfalso; exact (Lt.lt_not_le _ _ H1 H).
+    generalize (var_used_lift ctx c d v).
+    destruct (Compare_dec.lt_dec v c); tauto || omega. 
 Qed.
 
 Lemma has_type_lower : forall (ctx : context) (slot c d : nat) (t : term),
@@ -1287,32 +827,3 @@ Proof.
     rewrite IHctx.
     reflexivity.
 Qed.
-
-Lemma wf_ctx_no_zero : forall (ctx : context),
-    WF ctx ->
-    var_used ctx 0 ->
-    False
-.
-Proof.
-    intros ctx H; destruct H.
-    easy.
-    unfold push_var.
-    unfold lift1_context; simpl.
-    intro H1; destruct H1.
-    generalize H1; apply (lifting_destroys _ _ _ _ (le_0_n _) (PeanoNat.Nat.lt_0_succ _)).
-    generalize H1; apply (lifting_context_destroys _ _ _ _ (le_0_n _) (PeanoNat.Nat.lt_0_succ _)).
-    unfold push_var.
-    unfold lift1_context; simpl.
-    intro H1; destruct H1.
-    generalize H1; apply (lifting_destroys _ _ _ _ (le_0_n _) (PeanoNat.Nat.lt_0_succ _)).
-    generalize H1; apply (lifting_context_destroys _ _ _ _ (le_0_n _) (PeanoNat.Nat.lt_0_succ _)).
-    unfold push_var.
-    unfold lift1_context; simpl.
-    intro H1; destruct H1.
-    generalize H1; apply (lifting_destroys _ _ _ _ (le_0_n _) (PeanoNat.Nat.lt_0_succ _)).
-    generalize H1; apply (lifting_context_destroys _ _ _ _ (le_0_n _) (PeanoNat.Nat.lt_0_succ _)).
-    unfold push_dummy.
-    unfold lift1_context; simpl.
-    apply (lifting_context_destroys _ _ _ _ (le_0_n _) (PeanoNat.Nat.lt_0_succ _)).
-Qed.
- 
