verification/Im_Typing.v
@@ -1,0 +1,259 @@
+Require Import Program.Equality.
+
+Require List.
+Require Import Term.
+Require Import String.
+Require Import Context.
+Require Import ListLemmas.
+Require Import TermReduction.
+
+Reserved Notation "G |-im x := y" (at level 85, no associativity).
+
+(* Typing rules *)
+Inductive typing_im : context -> term -> term -> Prop :=
+(* Core typing *)
+| Im_TNat :
+    forall (ctx : context),
+    WF_im ctx ->
+    ctx |-im Nat := SmallKind
+| Im_TNatO : 
+    forall (ctx : context),
+    WF_im ctx ->
+    ctx |-im NatO := Nat
+| Im_TNatSucc : 
+    forall (ctx : context),
+    WF_im ctx ->
+    ctx |-im NatSucc := Forall "_"%string Nat Nat
+| Im_TNatRec : 
+    forall (ctx : context),
+    forall choice zero step num : term,
+    ctx |-im choice := Nat ===> SmallKind -> 
+    ctx |-im zero := App choice NatO ->
+    ctx |-im step := Forall "n"%string Nat (App (lift choice 0 1) (Var 0) ===> App (lift choice 0 2) (App NatSucc (Var 1))) ->
+    ctx |-im num := Nat ->
+    ctx |-im NatRec choice zero step num := App choice num
+| Im_TApp : 
+    forall (ctx : context),
+    forall (str : string) (domain range : term) (l r : term),
+    ctx |-im l := Forall str domain range ->
+    ctx |-im r := domain ->
+    ctx |-im App l r := top_subst range r
+| Im_TAbsSmall : 
+    forall (ctx : context),
+    forall (str : string) (range : term) (arg_type body : term),
+    ctx |-im arg_type := SmallKind ->
+    push_var ctx str arg_type |-im body := range ->
+    ctx |-im Abs str arg_type body := Forall str arg_type range
+| Im_TAbsType : 
+    forall (ctx : context),
+    forall (str : string) (range : term) (arg_type body : term) (i : nat),
+    ctx |-im arg_type := TypeKind i ->
+    { str == arg_type } :: ctx |-im body := range ->
+    ctx |-im Abs str arg_type body := Forall str arg_type range
+| Im_TAbsProp : 
+    forall (ctx : context),
+    forall (str : string) (range : term) (arg_type body : term),
+    ctx |-im arg_type := PropKind ->
+    { str == arg_type } :: ctx |-im body := range ->
+    ctx |-im Abs str arg_type body := Forall str arg_type range
+| Im_TVar : 
+    forall (ctx : context),
+    forall (n : nat) (t : term), 
+    WF_im ctx -> 
+    ctx[n] := t -> 
+    ctx |-im Var n := t
+| Im_TSmallKind : 
+    forall (ctx : context),
+    WF_im ctx -> 
+    ctx |-im SmallKind := TypeKind 0
+| Im_TPropKind :
+    forall (ctx : context),
+    WF_im ctx -> 
+    ctx |-im PropKind := TypeKind 0
+| Im_TTypeKind : 
+    forall (ctx : context),
+    WF_im ctx -> 
+    forall n : nat, ctx |-im TypeKind n := TypeKind (S n)
+| Im_TForallType : 
+    forall (ctx : context),
+    forall (str : string) (domain range : term) (universe : nat),
+    ctx |-im domain := TypeKind universe ->
+    { str == domain } :: ctx |-im range := TypeKind universe ->
+    ctx |-im Forall str domain range := TypeKind universe
+| Im_TForallPropSmall : 
+    forall (ctx : context),
+    forall (str : string) (domain range : term),
+    ctx |-im domain := SmallKind ->
+    { str == domain } :: ctx |-im range := PropKind ->
+    ctx |-im Forall str domain range := PropKind
+| Im_TForallPropProp : 
+    forall (ctx : context),
+    forall (str : string) (domain range : term),
+    ctx |-im domain := PropKind ->
+    { str == domain } :: ctx |-im range := PropKind ->
+    ctx |-im Forall str domain range := PropKind
+| Im_TForallPropType : 
+    forall (ctx : context),
+    forall (str : string) (domain range : term),
+    forall (i : nat), ctx |-im domain := TypeKind i ->
+    { str == domain } :: ctx |-im range := PropKind ->
+    ctx |-im Forall str domain range := PropKind
+| Im_TForallSmallSmall : 
+    forall (ctx : context),
+    forall (str : string) (domain range : term),
+    ctx |-im domain := SmallKind ->
+    { str == domain } :: ctx |-im range := SmallKind ->
+    ctx |-im Forall str domain range := SmallKind
+| Im_TForallSmallProp : 
+    forall (ctx : context),
+    forall (str : string) (domain range : term),
+    ctx |-im domain := PropKind ->
+    { str == domain } :: ctx |-im range := SmallKind ->
+    ctx |-im Forall str domain range := SmallKind
+(* Universe transition rules *)
+| Im_JumpToTypeUniverseSmall :
+    forall (ctx : context),
+    forall (t : term),
+    ctx |-im t := SmallKind ->
+    ctx |-im t := TypeKind 0
+| Im_JumpToTypeUniverseProp :
+    forall (ctx : context),
+    forall (t : term),
+    ctx |-im t := PropKind ->
+    ctx |-im t := TypeKind 0
+| Im_RaiseUniverse : 
+    forall (ctx : context),
+    forall (t : term) (universe : nat),
+    ctx |-im t := TypeKind universe ->
+    ctx |-im t := TypeKind (S universe)
+(* Conversion axioms *)
+| Im_ConversionSmallL : 
+    forall (ctx : context),
+    forall (t : term) (type type' : term),
+    ctx |-im t := type ->
+    ctx |-im type := SmallKind ->
+    type ->b type' ->
+    ctx |-im type' := SmallKind ->
+    ctx |-im t := type'
+| Im_ConversionPropL : 
+    forall (ctx : context),
+    forall (t : term) (type type' : term),
+    ctx |-im t := type ->
+    ctx |-im type := PropKind ->
+    type ->b type' ->
+    ctx |-im type' := PropKind ->
+    ctx |-im t := type'
+| Im_ConversionTypeL : 
+    forall (ctx : context),
+    forall (t : term) (type type' : term) (i : nat),
+    ctx |-im t := type ->
+    ctx |-im type := TypeKind i ->
+    type ->b type' ->
+    ctx |-im type' := TypeKind i ->
+    ctx |-im t := type'
+| Im_ConversionSmallR : 
+    forall (ctx : context),
+    forall (t : term) (type type' : term),
+    ctx |-im t := type ->
+    ctx |-im type := SmallKind ->
+    type' ->b type ->
+    ctx |-im type' := SmallKind ->
+    ctx |-im t := type'
+| Im_ConversionPropR : 
+    forall (ctx : context),
+    forall (t : term) (type type' : term),
+    ctx |-im t := type ->
+    ctx |-im type := PropKind ->
+    type' ->b type ->
+    ctx |-im type' := PropKind ->
+    ctx |-im t := type'
+| Im_ConversionTypeR : 
+    forall (ctx : context),
+    forall (t : term) (type type' : term) (i : nat),
+    ctx |-im t := type ->
+    ctx |-im type := TypeKind i ->
+    type' ->b type ->
+    ctx |-im type' := TypeKind i ->
+    ctx |-im t := type'
+| Im_ConversionSmallRename : 
+    forall (ctx : context),
+    forall (t : term) (type type' : term),
+    ctx |-im t := type ->
+    ctx |-im type := SmallKind ->
+    type =a type' ->
+    ctx |-im type' := SmallKind ->
+    ctx |-im t := type'
+| Im_ConversionPropRename : 
+    forall (ctx : context),
+    forall (t : term) (type type' : term),
+    ctx |-im t := type ->
+    ctx |-im type := PropKind ->
+    type =a type' ->
+    ctx |-im type' := PropKind ->
+    ctx |-im t := type'
+| Im_ConversionTypeRename : 
+    forall (ctx : context),
+    forall (t : term) (type type' : term) (i : nat),
+    ctx |-im t := type ->
+    ctx |-im type := TypeKind i ->
+    type =a type' ->
+    ctx |-im type' := TypeKind i ->
+    ctx |-im t := type'
+(*Refinement types!*)
+| Im_RefinementSmall :
+    forall (ctx : context),
+    forall (t condition : term) (type : term),
+    ctx |-im t := type ->
+    ctx |-im type := SmallKind ->
+    ctx |-im condition := type ===> PropKind ->
+    ctx |-im (Refine t condition) := SmallKind
+| Im_RefinementType :
+    forall (ctx : context),
+    forall (t condition : term) (type : term) (universe : nat),
+    ctx |-im t := type ->
+    ctx |-im type := TypeKind universe ->
+    ctx |-im condition := type ===> PropKind ->
+    ctx |-im (Refine t condition) := TypeKind universe
+(* Well formed context axioms *)
+with WF_im : context -> Prop :=
+| Im_WF_empty : WF_im nil
+| Im_WF_assum_small : 
+    forall (ctx : context) (str : string) (t : term),
+    WF_im ctx ->
+    ctx |-im t := SmallKind ->
+    WF_im (push_var ctx str t)
+| Im_WF_assum_prop :
+    forall (ctx : context) (str : string) (t : term),
+    WF_im ctx ->
+    ctx |-im t := PropKind ->
+    WF_im (push_var ctx str t)
+| Im_WF_assum_type :
+    forall (ctx : context) (str : string) (t : term) (i : nat),
+    WF_im ctx ->
+    ctx |-im t := TypeKind i ->
+    WF_im (push_var ctx str t)
+| Im_WF_dummy_assum :
+    forall (ctx : context),
+    WF_im ctx ->
+    WF_im (push_dummy ctx)
+
+where "G |-im x := y" := (typing_im G x y)
+.
+
+(* Induction scheme when the simple induction won't do the trick *)
+Scheme typing_im_ind_mut := Induction for 
+typing_im Sort Prop
+with wf_im_ind_mut := Induction for 
+WF_im Sort Prop.
+
+Definition typable (ctx : context) (t : term) := exists type : term, ctx |-im t := type.
+Notation "G |-im x := ?" := (typable G x) (at level 85, no associativity).
+
+Theorem typable_wf : forall (ctx : context) (t type : term),
+    ctx |-im t := type ->
+    WF_im ctx
+.
+Proof.
+    intros.
+    induction H; try easy.
+Qed.
